adding a lemma: upd_reg_preserves_match_state

proof/MatchState.v
@@ -64,7 +64,6 @@ Section S.
   Definition size_of_regs := 11 * 8. (**r we have 11 regs R0 - R10 *)
   Definition size_of_state (st: DxState.state) := 100 + 16 * (Z.of_nat (mrs_num st)).
 
-
 (**r
 Definition state_struct_def: Ctypes.composite_definition := 
   Ctypes.Composite state_id Ctypes.Struct [
@@ -76,6 +75,13 @@ Definition state_struct_def: Ctypes.composite_definition :=
   ] Ctypes.noattr.
 
 *)
+  
+Definition is_byte_memval (mv: memval): Prop :=
+  match mv with
+  | Undef => False
+  | Byte b => True
+  | Fragment _ _ _ => False
+  end.
 
   Record match_state  (st: DxState.state) (m: mem) : Prop :=
     {
@@ -86,7 +92,9 @@ Definition state_struct_def: Ctypes.composite_definition :=
       mrs_num  : Mem.loadv AST.Mint32 m (Vptr bl_state (Ptrofs.repr (size_of_regs + 8))) = Some (Vint  (Int.repr (Z.of_nat (DxState.mrs_num st)))) /\ (Z.of_nat(DxState.mrs_num st)) >= 1; (**r at least we have the memory region that corresponds to the input paramters of the interpreter *)
       mem_regs : match_regions (bpf_mrs st) bl_state (Ptrofs.repr (size_of_regs + 12)) m /\ List.length (bpf_mrs st) = (DxState.mrs_num st); (**r the number of bpf_mrs is exactly the mrs_num *)
       mperm    : Mem.range_perm m bl_state 0 (size_of_state st) Cur Freeable;
-      minvalid : ~Mem.valid_block (bpf_m st) bl_state /\ ~Mem.valid_block (bpf_m st) ins_block  (*forall chunk ofs p, ~Mem.valid_access (bpf_m st) chunk bl_state ofs p /\ ~Mem.perm (bpf_m st) bl_state ofs Cur p *)(**r ysh: bl_state doesn't exist in st *)
+      minvalid : ~Mem.valid_block (bpf_m st) bl_state /\ ~Mem.valid_block (bpf_m st) ins_block;  (**r ysh: bl_state and ins_block don't exist in st *)
+      munchange: Mem.unchanged_on (fun b _ => b <> bl_state /\ b <> ins_block) (bpf_m st) m; (**r (bpf_m st) = m - {bl_state, ins_block} *)
+      mByte    : forall b ofs, (b <> bl_state /\ b <> ins_block) -> is_byte_memval (Maps.ZMap.get ofs (Maps.PMap.get b (Mem.mem_contents m)));
     }.
 
 End S.
@@ -260,4 +268,180 @@ Proof.
   repeat rewrite <- UMOD by (simpl ; tauto).
   intuition.
 Qed.
+
+(**r a set of lemmas say upd_reg/flag/pc... don't change the memory of rbpf *)
+
+Lemma upd_reg_same_mem:
+  forall st0 r vl,
+    bpf_m st0 = bpf_m (DxState.upd_reg r vl st0).
+Proof.
+  unfold DxState.upd_reg.
+  intros.
+  reflexivity.
+Qed.
+
+Lemma upd_pc_same_mem:
+  forall st0 pc,
+    bpf_m st0 = bpf_m (DxState.upd_pc pc st0).
+Proof.
+  unfold DxState.upd_pc.
+  intros.
+  reflexivity.
+Qed.
+
+Lemma upd_pc_incr_same_mem:
+  forall st0,
+    bpf_m st0 = bpf_m (DxState.upd_pc_incr st0).
+Proof.
+  unfold DxState.upd_pc_incr.
+  intros.
+  reflexivity.
+Qed.
+
+Lemma upd_flag_same_mem:
+  forall st0 f,
+    bpf_m st0 = bpf_m (DxState.upd_flag f st0).
+Proof.
+  unfold DxState.upd_flag.
+  intros.
+  reflexivity.
+Qed.
+
+Lemma upd_unchanged_on:
+  forall st m0 m1 blk ins chunk ofs vl
+  (Hst    : match_state blk ins st m0)
+  (Hstore : Mem.store chunk m0 blk ofs vl = Some m1),
+    Mem.unchanged_on (fun b _ => b <> blk /\ b <> ins) m0 m1.
+Proof.
+  intros.
+  destruct Hst.
+  destruct minj0.
+  clear - mi_inj mi_freeblocks minvalid0 munchange0 mByte0 Hstore.
+  eapply Mem.store_unchanged_on.
+  rewrite Hstore.
+  reflexivity.
+  intros.
+  intro.
+  destruct H0.
+  apply H0; reflexivity.
+Qed.
+
+Lemma upd_reg_preserves_match_state:
+  forall st0 st1 m0 m1 blk ins r vl
+  (Hst    : match_state blk ins st0 m0)
+  (Hst1   : DxState.upd_reg r (Vlong vl) st0 = st1)
+  (Hstore : Mem.store AST.Mint64 m0 blk (8 + 8 * id_of_reg r) (Vlong vl) = Some m1),
+    match_state blk ins st1 m1.
+Proof.
+  intros.
+  set (Hst' := Hst).
+  destruct Hst'.
+  split; unfold Mem.loadv in *.
+  -
+    destruct minj0.
+    split.
+    + (**r mi_inj *)
+      clear - Hst Hst1 mi_inj mi_freeblocks minvalid0 munchange0 mByte0 Hstore.
+      destruct minvalid0 as (minvalid_st & minvalid_ins).
+      destruct mi_inj.
+
+      (**r say rbpf blocks are all Byte *)
+      unfold is_byte_memval in mByte0.
+
+      split; intros; inversion H; subst; rewrite <- (upd_reg_same_mem _ r (Vlong vl)) in H0.
+      * (**r mi_perm *)
+        specialize (mi_perm b2 b2 0 ofs k p H H0).
+        (**r Search (Mem.perm).*)
+        apply Mem.perm_store_1 with (chunk:= Mint64) (m1:= m0) (b:=blk) (ofs:=(8 + 8 * id_of_reg r)%Z) (v:= (Vlong vl)).
+        assumption.
+        assumption.
+      * (**r mi_align *)
+        apply Z.divide_0_r.
+      * (**r mi_memval *)
+        specialize (mi_memval b2 ofs b2 0 H H0).
+        destruct munchange0.
+
+        (***r Search (memval_inject). *)
+        repeat rewrite Z.add_0_r.
+        destruct (Pos.eqb b2 blk) eqn: Hblk_eq.
+        ** (**r b2 = blk *)
+          apply Peqb_true_eq in Hblk_eq.
+          subst b2.
+          apply mi_freeblocks in minvalid_st.
+          rewrite minvalid_st in H.
+          inversion H.
+        ** (**r b2 <> blk *)
+          destruct (Pos.eqb b2 ins) eqn: Hins_eq.
+          ++ (**r b2 = ins *)
+            apply Peqb_true_eq in Hins_eq.
+            subst b2.
+            apply mi_freeblocks in minvalid_ins.
+            rewrite minvalid_ins in H.
+            inversion H.
+          ++ (**r b2 <> ins *)
+            (**r Search (Pos.eqb). *)
+            rewrite Pos.eqb_neq in *.
+            assert (Hb2_neq: b2 <> blk /\ b2 <> ins). {
+              split; assumption.
+            }
+            specialize (unchanged_on_contents b2 ofs Hb2_neq H0).
+            rewrite <- (upd_reg_same_mem _ r (Vlong vl)).
+            rewrite <- unchanged_on_contents.
+            assert (Hunchange: Mem.unchanged_on (fun b _ => b <> blk /\ b <> ins) m0 m1). {
+              eapply upd_unchanged_on.
+              apply Hst.
+              apply Hstore.
+            }
+            destruct Hunchange.
+            (**r we need : Mem.perm m0 b2 ofs0 Cur Readable *)
+            assert (Hm0_perm: Mem.perm m0 b2 ofs Cur Readable). {
+              specialize (mi_perm b2 b2 0 ofs Cur Readable H H0).
+              rewrite Z.add_0_r in mi_perm.
+              assumption.
+            }
+            specialize (unchanged_on_contents0 b2 ofs Hb2_neq Hm0_perm).
+            rewrite unchanged_on_contents0.
+            specialize (mByte0 b2 ofs Hb2_neq).
+            destruct (Maps.ZMap.get _ (Maps.PMap.get _ (Mem.mem_contents _))) eqn: HByte in mByte0; [ inversion mByte0| idtac | inversion mByte0].
+            rewrite HByte.
+            constructor.
+    + (**r mi_freeblocks *)
+      intros.
+      subst.
+      rewrite <- (upd_reg_same_mem _ r (Vlong vl)) in H.
+      apply mi_freeblocks.
+      assumption.
+    + (**r mi_mappedblocks *)
+      intros.
+      assert (Hunchange: Mem.unchanged_on (fun b _ => b <> blk /\ b <> ins) m0 m1). {
+        eapply upd_unchanged_on; eauto.
+      }
+      eapply Mem.valid_block_unchanged_on; eauto.
+    + (**r mi_no_overlap *)
+      subst.
+      rewrite <- (upd_reg_same_mem _ r (Vlong vl)).
+      assumption.
+    + (**r mi_representable *)
+      subst.
+      rewrite <- (upd_reg_same_mem _ r (Vlong vl)).
+      assumption.
+    + (**r mi_perm_inv *)
+      subst.
+      rewrite <- (upd_reg_same_mem _ r (Vlong vl)).
+      intros.
+      eapply mi_perm_inv; eauto.
+      eapply Mem.perm_unchanged_on_2; eauto.
+      eapply upd_unchanged_on; eauto.
+      simpl.
+      inversion H; subst.
+      destruct minvalid0 as (minvalid_st & minvalid_ins).
+      split.
+      * specialize (mi_freeblocks _ minvalid_st); intro; subst; rewrite mi_freeblocks in H; inversion H.
+      * specialize (mi_freeblocks _ minvalid_ins); intro; subst; rewrite mi_freeblocks in H; inversion H.
+   -
+    eapply Mem.load_unchanged_on; eauto. admit.
+    eapply upd_unchanged_on; eauto.
+    intros; simpl.
+    split.
+
 Close Scope Z_scope.
